relating safety via different ext_specs

concurrency/semax_conc.v
@@ -1,4 +1,3 @@
-(*Require Import msl.rmaps. *)
 Require Import msl.msl_standard.
 Require Import msl.seplog.
 Require Import veric.base.
@@ -11,7 +10,11 @@ Require Import veric.tycontext.
 Require Import veric.expr2.
 Require Import veric.semax.
 Require Import veric.semax_call.
+Require Import veric.semax_ext.
 Require Import veric.semax_ext_oracle.
+Require Import veric.juicy_safety.
+Require Import veric.Clight_new.
+Require Import sepcomp.semantics.
 Require Import sepcomp.extspec.
 Require Import floyd.proofauto.
 
@@ -67,7 +70,6 @@ Definition Oracle := list rmap.
 
 (*+ Specification of each concurrent primitive *)
 
-(*
 Definition acquire_spec :=
    WITH v : val, sh : share, R : Pred
    PRE [ _lock OF tptr tlock ]
@@ -78,9 +80,8 @@ Definition acquire_spec :=
      PROP ()
      LOCAL ()
      SEP (lock_inv sh v (Interp R); lock_hold Share.top v; Interp R).
- *)
 
-Definition acquire_spec :=
+Definition acquire_oracular_spec :=
   mk_funspecOracle
     Oracle
     (* ARGS *)
@@ -109,7 +110,6 @@ Definition acquire_spec :=
          SEP (lock_inv sh v (Interp R); lock_hold Share.top v; Interp R)
        end).
 
-(*
 Definition release_spec :=
    WITH v : val, sh : share, R : Pred
    PRE [ _lock OF tptr tlock ]
@@ -120,9 +120,8 @@ Definition release_spec :=
      PROP ()
      LOCAL ()
      SEP (lock_inv sh v (Interp R)).
-*)
 
-Definition release_spec :=
+Definition release_oracular_spec :=
   mk_funspecOracle
     Oracle
     (* ARGS *)
@@ -236,46 +235,202 @@ Definition spawn_spec :=
 
 
 (*! The void ext_spec *)
-Definition void_spec : external_specification juicy_mem external_function (list rmap) :=
+Definition void_spec T : external_specification juicy_mem external_function T :=
     Build_external_specification
-      juicy_mem external_function (list rmap)
+      juicy_mem external_function T
       (fun ef => False)
       (fun ef Hef ge tys vl m z => False) 
       (fun ef Hef ge ty vl m z => False)
       (fun rv m z => False).
 
-Definition ok_void_spec : OracleKind.
- refine (Build_OracleKind (list rmap) (Build_juicy_ext_spec _ void_spec _ _ _)).
+Definition ok_void_spec (T : Type) : OracleKind.
+ refine (Build_OracleKind T (Build_juicy_ext_spec _ (void_spec T) _ _ _)).
 Proof.
   simpl; intros; contradiction.
   simpl; intros; contradiction.
   simpl; intros; intros ? ? ? ?; contradiction.
 Defined.
 
-Definition threadspecs (cs : compspecs) (ext_link : string -> ident) := 
-  (ext_link "acquire"%string, acquire_spec) ::
-  (ext_link "release"%string, release_spec) ::
+Definition concurrent_oracular_specs (cs : compspecs) (ext_link : string -> ident) := 
+  (ext_link "acquire"%string, acquire_oracular_spec) ::
+  (ext_link "release"%string, release_oracular_spec) ::
   nil.
 
-(*
-Definition threadspecs (cs : compspecs) (ext_link : string -> ident) :=
+Definition concurrent_specs (cs : compspecs) (ext_link : string -> ident) :=
   (ext_link "acquire"%string, acquire_spec) ::
   (ext_link "release"%string, release_spec) ::
-  (ext_link "makelock"%string, makelock_spec cs) ::
-  (ext_link "freelock"%string, freelock_spec cs) ::
-  (ext_link "spawn"%string, spawn_spec) ::
+  (* (ext_link "makelock"%string, makelock_spec cs) :: *)
+  (* (ext_link "freelock"%string, freelock_spec cs) :: *)
+  (* (ext_link "spawn"%string, spawn_spec) :: *)
   nil.
-*)
 
-Definition conc_ext_spec (cs : compspecs) (ext_link : string -> ident) :=
+Definition concurrent_oracular_ext_spec (cs : compspecs) (ext_link : string -> ident) :=
   add_funspecsOracle_rec
     ext_link
-    ok_void_spec.(@OK_ty)
-    ok_void_spec.(@OK_spec)
-    (threadspecs cs ext_link).
+    (ok_void_spec (list rmap)).(@OK_ty)
+    (ok_void_spec (list rmap)).(@OK_spec)
+    (concurrent_oracular_specs cs ext_link).
 
-Definition Concurrent_Espec cs ext_link := Build_OracleKind (list rmap) (conc_ext_spec cs ext_link).
+Definition concurrent_ext_spec Z (cs : compspecs) (ext_link : string -> ident) :=
+  add_funspecs_rec
+    ext_link
+    (ok_void_spec Z).(@OK_ty)
+    (ok_void_spec Z).(@OK_spec)
+    (concurrent_specs cs ext_link).
 
+Definition Concurrent_Oracular_Espec cs ext_link :=
+  Build_OracleKind
+    (list rmap)
+    (concurrent_oracular_ext_spec cs ext_link).
+
+Definition Concurrent_Espec Z cs ext_link :=
+  Build_OracleKind
+    Z
+    (concurrent_ext_spec Z cs ext_link).
+
+Lemma strong_nat_ind (P : nat -> Prop) (IH : forall n, (forall i, lt i n -> P i) -> P n) n : P n.
+Proof.
+  apply IH; induction n; intros i li; inversion li; eauto.
+Qed.
+
+Set Printing Implicit.
+Require Import sepcomp.step_lemmas.
+
+Lemma at_external_not_halted (G C M : Type) (csem : semantics.CoreSemantics G C M) (q : C) :
+  semantics.at_external csem q <> None -> semantics.halted csem q = None.
+Proof.
+  destruct (@semantics.at_external_halted_excl G C _ csem q); tauto.
+Qed.
+
+Theorem oracular_refinement cs ext_link ge n oracle c m :
+  jsafeN (Concurrent_Espec unit cs ext_link).(@OK_spec) ge n tt c m ->
+  jsafeN (Concurrent_Oracular_Espec cs ext_link).(@OK_spec) ge n oracle c m.
+Proof.
+  revert oracle c m; induction n as [n IH] using strong_nat_ind; intros oracle c m.
+  intros Safe; induction Safe as [ | | n Ω c m e sig args x E Pre Post | ].
+  all: swap 3 4.
+  - (* safeN_0 *)
+    now eapply safeN_0; eauto.
+  
+  - (* safeN_step *)
+    eapply safeN_step; eauto.
+    now apply IH; auto.
+  
+  - (* safeN_halted *)
+    now eapply safeN_halted; eauto.
+  
+  - (* safeN_external *)
+    destruct c as [ | ef_ sig_ args_ lid ve te k ]; [ discriminate | ].
+    simpl in E; injection E as -> -> -> .
+    
+    (* We need to know which of the externals we are talking about *)
+    (* paragraph below: ef has to be an EF_external *)
+    assert (Hef : match e with EF_external _ _ => True | _ => False end).
+    {
+      match goal with x : ext_spec_type _ _  |- _ => clear -x end.
+      destruct e eqn:Ee; [ apply I | .. ];
+        simpl in x;
+        repeat match goal with
+                 _ : context [ (* o_ *)ident_eq ?x ?y ] |- _ =>
+                 destruct ((* o_ *)ident_eq x y); try discriminate; try tauto
+               end.
+      all: match goal with E : _ = 1%positive |- _ => admit end.
+    }
+    
+    assert (Ex : exists name sig, e = EF_external name sig) by (destruct e; eauto; tauto).
+    destruct Ex as (name & sg & ->); clear Hef.
+    
+    Unset Printing Implicit.
+    Local Notation "{| 'JE_spec ... |}" := {| JE_spec := _; JE_pre_hered := _; JE_post_hered := _; JE_exit_hered := _ |}.
+    revert x Pre Post.
+    simpl (ext_spec_pre _); simpl (ext_spec_post _); simpl (ext_spec_type _).
+    unfold funspec2pre, funspec2post, ext_spec_type, ext_spec_pre, ext_spec_post.
+    destruct (ident_eq (ext_link "acquire"%string) (ef_id ext_link (EF_external name sg)))
+      as [ H_acquire | notacquire ].
+    
+    { (* case 1 : acquire *)
+      intros [phi_x [[vx shx] Rx]] Pre Post.
+      destruct oracle as [ | phi_oracle oracle ].
+      - simpl.
+        
+        (* this is the x parameter for the WITH clause, but it has the wrong type. *)
+        pose (xwith := (phi_x, (False, @nil rmap, vx, shx, Rx))).
+        assert ((rmap * (Prop * list rmap * val * share * Pred) =
+                 @ext_spec_type
+                   juicy_mem external_function (@OK_ty (Concurrent_Oracular_Espec cs ext_link))
+                   (@OK_spec (Concurrent_Oracular_Espec cs ext_link)) (EF_external name sg))
+               )%type as EqT.
+        { simpl. rewrite H_acquire. simpl. if_tac;[ reflexivity | congruence ]. }
+        
+        (* getting a JM copy of x of the correct type *)
+        remember xwith as x2.
+        assert (JMeq xwith x2). subst. apply JMeq_refl.
+        clear Heqx2.
+        revert x2 H.
+        pattern (rmap * (Prop * list rmap * val * share * Pred))%type at 1 3.
+        cut (
+            (fun T : Type =>
+               forall x2 : T,
+                 @JMeq (rmap * (Prop * list rmap * val * share * Pred)) xwith T x2 ->
+                 @jsafeN (list rmap) (concurrent_oracular_ext_spec cs ext_link) ge (S n) []
+                         (Clight_new.ExtCall (EF_external name sg) sig args lid ve te k) m)
+              (@ext_spec_type juicy_mem external_function (@OK_ty (Concurrent_Oracular_Espec cs ext_link))
+                              (@OK_spec (Concurrent_Oracular_Espec cs ext_link)) (EF_external name sg))).
+        {
+          assert (APP : forall P Q  : Prop, P = Q -> P -> Q) by (intros ? ? -> ; auto).
+          apply APP.
+          rewrite <- EqT.
+          reflexivity.
+        }
+        intros x2 E2.
+        
+        Set Printing All.
+        (* the following is strange, it fails to typecheck even though
+        it is provided as a quote from one of the types *)
+        Fail 
+          set (qwdq := @ext_spec_type juicy_mem external_function (list rmap)
+                                      (JE_spec (list rmap) (concurrent_oracular_ext_spec cs ext_link))
+                                      acquire_oracular_spec).
+        
+        Fail apply safeN_external with
+        (e := acquire_oracular_spec)
+          (x := x2).
+        
+        (* solve this with JM_eq + ident_eq (or ) *)
+        
+        Set Printing Implicit.
+        eapply (@safeN_external
+                  genv Clight_new.corestate juicy_mem Oracle (@Genv.genv_symb _ _) Hrel
+                  (juicy_core_sem cl_core_sem)
+                  (@OK_spec (Concurrent_Oracular_Espec cs ext_link))
+                  ge n
+               )
+        .
+        + reflexivity.
+        + admit.
+        + admit.
+      
+      - (* oracle not empty... *)
+        admit.
+    }
+    
+    unfold JE_spec.
+    unfold funspec2jspec, funspec2extspec.
+    simpl (ext_spec_pre _); simpl (ext_spec_post _); simpl (ext_spec_type _).
+    unfold funspec2pre, funspec2post, ext_spec_type, ext_spec_pre, ext_spec_post, release_spec.
+    
+    destruct (ident_eq (ext_link "release"%string) (ef_id ext_link (EF_external name sg)))
+      as [ H_release | notrelease ].
+    { (* case 2: release *)
+      admit.
+    }
+    
+    { (* remaining of cases *)
+      intros x; exfalso; tauto.
+    }
+Admitted.
+
+(*
 Lemma semax_conc' cs (ext_link: string -> ident) id sig cc A P Q :
   let fs := threadspecs cs ext_link in
   let f := mk_funspecOracle Oracle sig cc A P Q in
@@ -303,3 +458,4 @@ Proof.
   subst.
   apply semax_conc'; hnf; auto.
 Qed.
+ *)
